examples/low-level/crypto/Crypto.Symmetric.Poly1305.Bignum.Lemmas.Part2.fst
@@ -1,0 +1,333 @@
+module Crypto.Symmetric.Poly1305.Bignum.Lemmas.Part2
+
+open FStar.Mul
+open FStar.Ghost
+(** Machine integers *)
+open FStar.UInt64
+(** Effects and memory layout *)
+open FStar.HyperStack
+open FStar.HST
+(** Buffers *)
+open FStar.Buffer
+(** Mathematical definitions *)
+open Math.Axioms
+open Math.Lib
+open Math.Lemmas
+
+open Crypto.Symmetric.Poly1305.Parameters
+open Crypto.Symmetric.Poly1305.Bigint
+open Crypto.Symmetric.Poly1305.Bignum.Lemmas.Part1
+
+module U32 = FStar.UInt32
+module U64 = FStar.UInt64
+module HS = FStar.HyperStack
+
+
+#reset-options "--z3timeout 5 --initial_fuel 0 --max_fuel 0"
+
+let isDegreeReduced (h0:mem) (h1:mem) (b:bigint) =
+  live h0 b /\ live h1 b /\ length b >= 2*norm_length-1
+  /\ v (get h1 b 0) = v (get h0 b 0) + 5 * v (get h0 b 5)
+  /\ v (get h1 b 1) = v (get h0 b 1) + 5 * v (get h0 b 6)
+  /\ v (get h1 b 2) = v (get h0 b 2) + 5 * v (get h0 b 7)
+  /\ v (get h1 b 3) = v (get h0 b 3) + 5 * v (get h0 b 8)
+  /\ v (get h1 b 4) = v (get h0 b 4)
+
+let satisfiesModuloConstraints (h:heap) (b:bigint) : GTot Type0 =
+  live h b /\ length b >= 2*norm_length-1
+  /\ maxValue h b (2*norm_length-1) * 6 < pow2 63
+
+val lemma_freduce_degree_0:
+  h:mem ->
+  b:bigint ->
+  Lemma (requires (satisfiesModuloConstraints h b))
+	(ensures  (satisfiesModuloConstraints h b
+	  /\ 5 * v (get h b 5) < pow2 64 /\ 5 * v (get h b 6) < pow2 64 /\ 5 * v (get h b 7) < pow2 64
+	  /\ 5 * v (get h b 7) < pow2 64 /\ 5 * v (get h b 8) < pow2 64
+	  /\ v (get h b 0) + 5 * v (get h b 5) < pow2 64 /\ v (get h b 1) + 5 * v (get h b 6) < pow2 64
+	  /\ v (get h b 2) + 5 * v (get h b 7) < pow2 64 /\ v (get h b 3) + 5 * v (get h b 8) < pow2 64
+	))
+let lemma_freduce_degree_0 h b =
+  pow2_double_sum 63;
+  maxValue_lemma_aux h b (2*norm_length-1)
+
+
+let bound63 (h:heap) (b:bigint) : GTot Type0 =
+  live h b /\ v (get h b 0) < pow2 63 /\ v (get h b 1) < pow2 63 /\ v (get h b 2) < pow2 63
+  /\ v (get h b 3) < pow2 63 /\ v (get h b 4) < pow2 63
+
+
+#reset-options "--z3timeout 5 --initial_fuel 0 --max_fuel 0"
+
+val lemma_freduce_degree1:
+  h0:mem -> h1:mem ->
+  b:bigint ->
+  Lemma (requires (satisfiesModuloConstraints h0 b /\ isDegreeReduced h0 h1 b))
+	(ensures  (satisfiesModuloConstraints h0 b /\ isDegreeReduced h0 h1 b
+	  /\ bound63 h1 b))
+let lemma_freduce_degree1 h0 h1 b =
+  maxValue_lemma_aux h0 b (2*norm_length-1)
+
+
+#reset-options "--z3timeout 5 --initial_fuel 0 --max_fuel 0"
+
+assume val lemma_modulo_9: a:nat -> b:nat -> c:nat -> d:nat -> e:nat -> f:nat -> g:nat -> h:nat -> i:nat ->
+  Lemma (requires (True))
+	(ensures  (let p = reveal prime in
+	  (a + pow2 26 * b + pow2 52 * c + pow2 78 * d + pow2 104 * e
+	   + pow2 130 * f + pow2 156 * g + pow2 182 * h + pow2 208 * i ) % p
+	  = (a + pow2 26 * b + pow2 52 * c + pow2 78 * d + pow2 104 * e
+	     + (pow2 130 % p) * f + (pow2 156 % p) * g + (pow2 182 % p) * h + (pow2 208 % p) * i) % p))
+
+assume val lemma_modulo_mul: a:nat -> b:nat -> p:pos ->
+  Lemma (let p = reveal prime in (a * b) % p = (a%p * b) % p)
+
+assume val lemma_2_130_modulo_prime: unit -> Lemma (pow2 130 % (pow2 130 - 5) = 5)
+
+let lemma_modulo_00 (a:nat) (b:pos) : Lemma (requires (a < b)) (ensures ( a % b = a )) = ()
+let lemma_mul_nat (a:nat) (b:nat) : Lemma (a * b >= 0) = ()
+
+let lemma_pow2_modulo_prime0 () :
+  Lemma (let p = reveal prime in (
+    (5 * pow2 26) % p = 5 * pow2 26
+    /\ (5 * pow2 52) % p = 5 * pow2 52
+    /\ (5 * pow2 78) % p = 5 * pow2 78))
+  = assert_norm (pow2 3 = 8);
+    lemma_2_130_modulo_prime ();
+    let p = reveal prime in
+    pow2_plus 3 26;
+    pow2_plus 3 52;
+    pow2_plus 3 78;
+    pow2_double_sum 129;
+    pow2_lt_compat 129 5;
+    pow2_lt_compat 129 29;
+    pow2_lt_compat 129 55;
+    pow2_lt_compat 129 81;
+    lemma_modulo_00 (5 * pow2 26) p;
+    lemma_modulo_00 (5 * pow2 52) p;
+    lemma_modulo_00 (5 * pow2 78) p
+
+
+let lemma_pow2_modulo_prime () : Lemma (let p = reveal prime in
+  pow2 130 % p = 5 /\ pow2 156 % p = 5 * pow2 26
+  /\ pow2 182 % p = 5 * pow2 52 /\ pow2 208 % p = 5 * pow2 78)
+  = pow2_plus 130 26;
+    pow2_plus 130 52;
+    pow2_plus 130 78;
+    let p = reveal prime in
+    lemma_modulo_mul (pow2 130) (pow2 26) p;
+    lemma_modulo_mul (pow2 130) (pow2 52) p;
+    lemma_modulo_mul (pow2 130) (pow2 78) p;
+    lemma_pow2_modulo_prime0 ();
+    lemma_2_130_modulo_prime ()
+
+let lemma_2_26_p (a:nat) : Lemma (requires (a < pow2 26)) (ensures  (a < reveal prime /\ a % reveal prime = a))
+  = pow2_double_sum 129;
+    assert_norm(pow2 3 = 8);
+    pow2_lt_compat 129 3;
+    pow2_lt_compat 129 26;
+    lemma_modulo_00 a (reveal prime)
+
+
+#reset-options "--z3timeout 20 --initial_fuel 0 --max_fuel 0"
+
+val lemma_freduce_degree2:
+  h0:mem -> h1:mem ->
+  b:bigint ->
+  Lemma (requires (isDegreeReduced h0 h1 b))
+	(ensures  (isDegreeReduced h0 h1 b
+	  /\ eval h1 b norm_length % reveal prime = eval h0 b (2*norm_length-1) % reveal prime))
+let lemma_freduce_degree2 h0 h1 b =
+  let b0 = v (get h0 b 0) in
+  let b1 = v (get h0 b 1) in
+  let b2 = v (get h0 b 2) in
+  let b3 = v (get h0 b 3) in
+  let b4 = v (get h0 b 4) in
+  let b5 = v (get h0 b 5) in
+  let b6 = v (get h0 b 6) in
+  let b7 = v (get h0 b 7) in
+  let b8 = v (get h0 b 8) in
+  lemma_eval_bigint_9 h0 b;
+  let p = reveal prime in
+  cut(eval h0 b (2*norm_length-1) % p =
+      (b0 + pow2 26 * b1 + pow2 52 * b2 + pow2 78 * b3 + pow2 104 * b4
+      + pow2 130 * b5 + pow2 156 * b6 + pow2 182 * b7 + pow2 208 * b8) % p);
+  lemma_eval_bigint_5 h1 b;
+  lemma_mul_nat (pow2 26)  b1;
+  lemma_mul_nat (pow2 52)  b2;
+  lemma_mul_nat (pow2 78)  b3;
+  lemma_mul_nat (pow2 104) b4;
+  lemma_mul_nat (pow2 130) b5;
+  lemma_mul_nat (pow2 156) b6;
+  lemma_mul_nat (pow2 182) b7;
+  lemma_mul_nat (pow2 208) b8;
+  lemma_modulo_9 b0 b1 b2 b3 b4 b5 b6 b7 b8;
+  distributivity_add_right (pow2 26) b1 (5*b6);
+  distributivity_add_right (pow2 52) b2 (5*b7);
+  distributivity_add_right (pow2 78) b3 (5*b8);
+  let p = reveal prime in
+  lemma_modulo_mul (pow2 130) b5 p;
+  lemma_modulo_mul (pow2 156) b6 p;
+  lemma_modulo_mul (pow2 182) b7 p;
+  lemma_modulo_mul (pow2 208) b8 p;
+  lemma_pow2_modulo_prime ();
+  assert(eval h0 b (2*norm_length-1) % p =
+    (b0 + pow2 26 * b1 + pow2 52 * b2 + pow2 78 * b3 + pow2 104 * b4
+     + 5 * b5 + 5 * pow2 26 * b6 + 5 * pow2 52 * b7 + 5 * pow2 78 * b8) % p)
+
+val lemma_freduce_degree:
+  h0:mem ->
+  h1:mem ->
+  b:bigint ->
+  Lemma (requires (satisfiesModuloConstraints h0 b /\ isDegreeReduced h0 h1 b))
+	(ensures  (satisfiesModuloConstraints h0 b /\ isDegreeReduced h0 h1 b
+	  /\ bound63 h1 b
+	  /\ eval h1 b norm_length % reveal prime = eval h0 b (2*norm_length-1) % reveal prime))
+let lemma_freduce_degree h0 h1 b =
+  lemma_freduce_degree1 h0 h1 b;
+  lemma_freduce_degree2 h0 h1 b
+
+#reset-options "--z3timeout 20 --initial_fuel 0 --max_fuel 0"
+
+let isCarried (h0:mem) (h1:mem) (b:bigint) : GTot Type0 =
+  live h0 b /\ live h1 b /\ length b >= norm_length+1
+  /\ (
+      let b0 = v (get h0 b 0) in
+      let b1 = v (get h0 b 1) in
+      let b2 = v (get h0 b 2) in
+      let b3 = v (get h0 b 3) in
+      let b4 = v (get h0 b 4) in
+      let r0  = b0 / pow2 26 in
+      let r1  = (b1 + r0) / pow2 26 in
+      let r2  = (b2 + r1) / pow2 26 in
+      let r3  = (b3 + r2) / pow2 26 in
+      v (get h1 b 5) = (b4 + r3) / pow2 26
+      /\ v (get h1 b 0) = b0 % pow2 26
+      /\ v (get h1 b 1) = (b1 + r0)  % pow2 26
+      /\ v (get h1 b 2) = (b2 + r1)  % pow2 26
+      /\ v (get h1 b 3) = (b3 + r2)  % pow2 26
+      /\ v (get h1 b 4) = (b4 + r3)  % pow2 26
+    )
+
+#reset-options "--z3timeout 20 --initial_fuel 0 --max_fuel 0"
+
+
+let u633 = x:U64.t{v x < pow2 63}
+
+#reset-options "--z3timeout 5 --initial_fuel 0 --max_fuel 0"
+
+
+let isCarried_
+  (h1:mem)
+  (b0:U64.t) (b1:U64.t) (b2:U64.t) (b3:U64.t) (b4:U64.t)
+  (b:bigint) : GTot Type0 =
+  live h1 b /\ length b >= norm_length+1
+  /\ (
+      let r0  = v b0 / pow2 26 in
+      let r1  = (v b1 + r0) / pow2 26 in
+      let r2  = (v b2 + r1) / pow2 26 in
+      let r3  = (v b3 + r2) / pow2 26 in
+      v (get h1 b 5) = (v b4 + r3) / pow2 26
+      /\ v (get h1 b 0) = v b0 % pow2 26
+      /\ v (get h1 b 1) = (v b1 + r0)  % pow2 26
+      /\ v (get h1 b 2) = (v b2 + r1)  % pow2 26
+      /\ v (get h1 b 3) = (v b3 + r2)  % pow2 26
+      /\ v (get h1 b 4) = (v b4 + r3)  % pow2 26
+    )
+
+
+let carried_1 (h:mem) (b:bigint) : GTot Type0 =
+  live h b /\ length b >= norm_length+1
+  /\ v (get h b 0) < pow2 26
+  /\ v (get h b 1) < pow2 26
+  /\ v (get h b 2) < pow2 26
+  /\ v (get h b 3) < pow2 26
+  /\ v (get h b 4) < pow2 26
+  /\ v (get h b 5) <= pow2 38
+
+(* WIP *)
+
+assume val lemma_carry_1:
+  h0:mem -> h1:mem ->
+  b:bigint{length b >= norm_length+1} ->
+  Lemma (requires (bound63 h0 b /\ isCarried h0 h1 b))
+	(ensures  (bound63 h0 b /\ isCarried h0 h1 b
+	  /\ eval h1 b (norm_length+1) = eval h0 b norm_length /\ carried_1 h1 b))
+
+
+let carried_2 (h:mem) (b:bigint) : GTot Type0 =
+  live h b /\ length b >= norm_length+1
+  /\ v (get h b 0) < pow2 42
+  /\ v (get h b 1) < pow2 26
+  /\ v (get h b 2) < pow2 26
+  /\ v (get h b 3) < pow2 26
+  /\ v (get h b 4) < pow2 26
+
+
+let carried_3 (h:mem) (b:bigint) : GTot Type0 =
+  norm h b /\ length b >= norm_length+1
+  /\ v (get h b 5) <= 1
+  /\ (v (get h b 5) = 1
+    ==> (v (get h b 1) < pow2 18 /\ v (get h b 2) < pow2 18  /\ v (get h b 3) < pow2 18
+	/\ v (get h b 4) < pow2 18))
+
+assume val lemma_carry_2:
+  h0:mem -> h1:mem ->
+  b:bigint{length b >= norm_length+1} ->
+  Lemma (requires (carried_2 h0 b /\ isCarried h0 h1 b))
+	(ensures  (carried_2 h0 b /\ isCarried h0 h1 b
+	  /\ eval h1 b (norm_length+1) = eval h0 b norm_length
+	  /\ carried_3 h1 b))
+
+let carriedTopBottom (h0:mem) (h1:mem) (b:bigint) : GTot Type0 =
+  live h0 b /\ live h1 b /\ length b >= norm_length+1
+  /\ v (get h1 b 0) = v (get h0 b 0) + 5 * v (get h0 b 5)
+  /\ v (get h1 b 1) = v (get h0 b 1)
+  /\ v (get h1 b 2) = v (get h0 b 2)
+  /\ v (get h1 b 3) = v (get h0 b 3)
+  /\ v (get h1 b 4) = v (get h0 b 4)
+
+
+assume val lemma_carry_top_1:
+  h0:mem -> h1:mem ->
+  b:bigint ->
+  Lemma (requires (carried_1 h0 b /\ carriedTopBottom h0 h1 b))
+	(ensures  (carried_1 h0 b /\ carriedTopBottom h0 h1 b
+	  /\ carried_2 h1 b
+	  /\ eval h1 b norm_length % reveal prime = eval h0 b (norm_length+1) % reveal prime))
+
+
+let carried_4 (h:mem) (b:bigint) : GTot Type0 =
+  live h b /\ v (get h b 0) < pow2 26 + 5
+  /\ v (get h b 1) < pow2 26
+  /\ (v (get h b 0) >= pow2 26 ==> v (get h b 1) < pow2 18)
+  /\ v (get h b 2) < pow2 26
+  /\ v (get h b 3) < pow2 26
+  /\ v (get h b 4) < pow2 26
+
+
+assume val lemma_carry_top_2:
+  h0:mem -> h1:mem ->
+  b:bigint ->
+  Lemma (requires (norm h0 b /\ length b >= norm_length + 1
+		  /\ v (get h0 b 5) <= 1 /\ carriedTopBottom h0 h1 b))
+	(ensures  (norm h0 b /\ length b >= norm_length + 1
+	  /\ v (get h0 b 5) <= 1 /\ carriedTopBottom h0 h1 b
+	  /\ eval h1 b norm_length % reveal prime = eval h0 b (norm_length+1) % reveal prime
+	  /\ carried_4 h1 b))
+
+
+let isCarried01 (h0:mem) (h1:mem) (b:bigint) =
+  live h0 b /\ live h1 b
+  /\ v (get h1 b 0) = v (get h0 b 0) % pow2 26
+  /\ v (get h1 b 1) = v (get h0 b 1) + (v (get h0 b 0) / pow2 26)
+  /\ v (get h1 b 2) = v (get h0 b 2)
+  /\ v (get h1 b 3) = v (get h0 b 3)
+  /\ v (get h1 b 4) = v (get h0 b 4)
+
+assume val lemma_carry_0_to_1:
+  h0:mem -> h1:mem ->
+  b:bigint ->
+  Lemma (requires (carried_4 h0 b /\ isCarried01 h0 h1 b))
+	(ensures  (carried_4 h0 b /\ isCarried01 h0 h1 b
+	  /\ norm h1 b /\ eval h1 b norm_length = eval h0 b norm_length))
